defined addition of two vectors

src/nalgebra.lean
@@ -1,1 +1,18 @@
-#eval "Hello, world!"
+structure Vector (n : Nat) (α : Type u) where
+   data : Array α
+   prf : data.size = n
+
+def map {n : Nat} {α β: Type u} (f : α → β) (xs : Vector n α) :=
+  Vector.mk (Array.map f xs.data) rfl
+
+theorem zipWithSizeProof {α β γ : Type u} (xs : Array α) (ys : Array β) (f : α → β → γ) : (Array.zipWith xs ys f).size = xs.size := by
+  induction xs.data with
+  | nil => simp [Array.zipWith]; simp [Array.zipWithAux]; _
+  | cons x rest ih => _
+
+def zipWith {n : Nat} {α β γ : Type u} (xs : Vector n α) (ys : Vector n β) (f : α → β → γ) : Vector n γ :=
+  let zs₀ := Array.zipWith xs.data ys.data f
+  let prf : zs₀.size = n := by
+    simp [zipWithSizeProof xs.data ys.data f]
+    simp [xs.prf]
+  Vector.mk zs₀ prf
